Update wbw to work with new api
@jadephilipoom the remaining context to prove is in
src/Arithmetic/MontgomeryReduction/WordByWord/Definition.v and
src/Arithmetic/MontgomeryReduction/WordByWord/Proofs.v:
```coq
  Local Notation conditional_subtract_cps := (@drop_high_cps
R_numlimbs).
  (*Axiom conditional_subtract_cps : T (S R_numlimbs) -> forall {cpsT},
(T R_numlimbs -> cpsT) -> cpsT *)(* computes [arg - N] if [R <= arg],
and drops high bit *)
  Axiom conditional_subtract : T (S R_numlimbs) -> T R_numlimbs (*
computes [arg - N] if [R <= arg], and drops high bit *).
  Local Lemma small_add : forall n a b, small a -> small b -> small
(@add n a b).
  Proof.
    intros; apply Saturated.small_add; auto; try lia.
    cbv [uweight].
    rewrite ?Znat.Nat2Z.inj_succ, ?Z.pow_succ_r by lia.
    try nia.
  Admitted.
  Local Lemma small_add' : forall n a b, small a -> small b -> small
(@add' n a b).
  Proof.
    intros; apply Saturated.small_add; auto; try lia.
    cbv [uweight].
    rewrite !Znat.Nat2Z.inj_succ, !Z.pow_succ_r by lia.
    try nia.
  Admitted.
  Axiom conditional_subtract_cps_id : forall v cpsT f,
@conditional_subtract_cps v cpsT f = f (@conditional_subtract _ v).
  Axiom small_scmul : forall (n : nat) (a : Z) (v : T n),
      small v -> 0 <= a < Z.pos r -> 0 <= eval v < R -> small (scmul a
v).
  Axiom eval_conditional_subtract
    : forall v : T (S R_numlimbs),
      small v ->
      0 <= eval v < eval N + Z.pos R ->
      eval (conditional_subtract v) = eval v + (if Z.pos R <=? eval v
then - eval N else 0).
  Axiom small_conditional_subtract
    : forall v : T (S R_numlimbs),
      small v ->
      0 <= eval v < eval N + Z.pos R ->
      small (conditional_subtract v).
```

src/Arithmetic/MontgomeryReduction/WordByWord/Abstract/Dependent/Definition.v
@@ -25,6 +25,7 @@ Section WordByWordMontgomery.
     {add : forall {n}, T n -> T n -> T (S n)} (* joins carry *)
     {add' : forall {n}, T (S n) -> T n -> T (S (S n))} (* joins carry *)
     {drop_high : T (S (S R_numlimbs)) -> T (S R_numlimbs)} (* drops the highest limb *)
+    {conditional_subtract : T (S R_numlimbs) -> T R_numlimbs} (* computes [arg - N] if [R <= arg], and drops high bit *)
     (N : T R_numlimbs).
 
   (* Recurse for a as many iterations as A has limbs, varying A := A, S := 0, r, bounds *)
@@ -60,8 +61,11 @@ Section WordByWordMontgomery.
          | S count' => fun A_S => redc_loop count' (redc_body A_S)
          end.
 
-    Definition redc : T (S R_numlimbs)
+    Definition pre_redc : T (S R_numlimbs)
       := snd (redc_loop A_numlimbs (A, zero (1 + R_numlimbs))).
+
+    Definition redc : T R_numlimbs
+      := conditional_subtract pre_redc.
   End loop.
 End WordByWordMontgomery.
 
